theories/Syntax/UntypedReduction.v
@@ -2,63 +2,11 @@
 From Stdlib Require Import CRelationClasses.
 From LogRel Require Import Utils AutoSubst.Extra Notations.
 From Equations Require Import Equations. (* for depelim *)
-From LogRel.Syntax Require Import BasicAst Context NormalForms (* Weakening *) Computations.
+From LogRel.Syntax Require Import BasicAst Context NormalForms Weakening Computations.
 
 (** ** Reductions *)
 
 (** *** One-step reduction. *)
-
-Fixpoint whns_all {red : term -> term -> Type} (Pred : forall t t', red t t' -> Type)
-  {k v t} (w : @whns red k v t) {struct w} : Type :=
-  match w with
-  | whns_tEval notink => unit
-  | whns_tApp w => whns_all Pred w
-  | whns_tNatElim w => whns_all Pred w
-  | whns_tBoolElim w => whns_all Pred w
-  | whns_tEmptyElim w => whns_all Pred w
-  | whns_tTreeElim w => whns_all Pred w
-  | whns_tFst w => whns_all Pred w
-  | whns_tSnd w => whns_all Pred w
-  | whns_tIdElim w => whns_all Pred w
-  | whns_tAlpha w => whns_all Pred w
-  | whns_tXi w => whns_all Pred w
-  | whns_tXXi w => whns_all Pred w
-  | whns_tXXiRed w notink' r w'=> whns_all Pred w × Pred _ _ r × whns_all Pred w'
-  end.
-
-Fixpoint whns_all_forall red Pred : (forall t t' (r : red t t'), Pred _ _ r) ->
-  forall k v t (w : @whns red k v t), whns_all Pred w.
-Proof.
-  intros allr k v t w.
-  destruct w.
-  2-12: cbn; eapply whns_all_forall, allr.
-  + constructor.
-  + repeat constructor.
-    - eapply whns_all_forall, allr.
-    - eapply allr.
-    - eapply whns_all_forall, allr.
-Defined.
-
-
-Inductive closure (R : term -> term -> Type) : term -> term -> Type :=
-  | clos_nil t : closure R t t
-  | clos_cons t t' u : closure R t' u -> R t t' -> closure R t u.
-
-Fixpoint closure_all {R : term -> term -> Type} (PR : forall t t', R t t' -> Type)
-  {t t'} (rtt' : closure R t t') {struct rtt'} : Type :=
-  match rtt' with
-  | clos_nil _ t => unit
-  | clos_cons _ t t' u rt'u rtt' => closure_all PR rt'u × PR _ _ rtt'
-  end.
-
-Fixpoint closure_all_forall R PR : (forall t t' (rtt' : R t t'), PR _ _ rtt') -> forall t t' (rtt' : closure R t t'), closure_all PR rtt'.
-Proof.
-  intros allr t t' rtt'.
-  destruct rtt'; constructor.
-  - eapply closure_all_forall, allr.
-  - eapply allr.
-Defined.
-
 
 
 Inductive OneRedAlg {L : list ell} : term -> term -> Type :=
@@ -116,107 +64,45 @@ Inductive OneRedAlg {L : list ell} : term -> term -> Type :=
   [ L |tIdElim A x P hr y e ⤳ tIdElim A x P hr y e' ]
 | evalRel v k b (ℓ : ell) : in_ell ℓ k b ->
   [ L |tApp (tEval ℓ (tRel v)) (nat_to_term k) ⤳ (bool_to_term b) ]
-| evalBox ℓ ℓ' t : [ L | tEval ℓ (tBox ℓ' t) ⤳ t]
-| xiSubst ℓ n n' k : [L | n ⤳ n'] -> [L | tXi ℓ (nSucc k n) ⤳ tXi ℓ (nSucc k n')]
-| xiLeaf ℓ n : [L | tXi ℓ (nat_to_term n) ⤳ tLeaf (nat_to_term n) ]
-| xiNode (ℓ : ell) n (k : newnat ℓ) : whns (red := closure OneRedAlg) k 0 n ->
+| evalBox {ℓ ℓ' t} : [ L | tEval ℓ (tBox ℓ' t) ⤳ t]
+| xiSubst {ℓ n n' k} : [L | n ⤳ n'] -> [L | tXi ℓ (nSucc k n) ⤳ tXi ℓ (nSucc k n')]
+| xiLeaf {ℓ n }: [L | tXi ℓ (nat_to_term n) ⤳ tLeaf (nat_to_term n) ]
+| xiNode {ℓ : ell} {n} {k : newnat ℓ} : whne (ellNe k 0) n ->
   [L |tXi ℓ n ⤳ tNode (nat_to_term k) (tXi (cons_ell ℓ k true) n) (tXi (cons_ell ℓ k false) n) ]
-| xxiSubst ℓ m m' n k : [L | m ⤳ m'] -> [L | tXXi ℓ (nSucc k m) n ⤳ tXXi ℓ (nSucc k m') n]
+| xxiSubst {ℓ m m' n k} : [L | m ⤳ m'] -> [L | tXXi ℓ (nSucc k m) n ⤳ tXXi ℓ (nSucc k m') n]
+| xxiLeaf {ℓ k n} : [L | tXXi ℓ (nat_to_term k) n ⤳ tRefl tTree (tLeaf (nat_to_term k)) ]
+| xxiNode {ℓ : ell} {m n} {k : newnat ℓ} (ℓt := cons_ell ℓ k true) (ℓf := cons_ell ℓ k false) : whne (ellNe k 0) m ->
+  [L | tXXi ℓ m n ⤳
+    tEllElim k ℓ (tId tNat (dEval (tXi ℓ m⟨upRen_term_term ↑⟩) (tRel 0)) m)
+      (tXXi ℓt m⟨upRen_term_term ↑⟩⟨upRen_term_term ↑⟩[(tBox ℓ (tEval ℓt (tRel 0)))..] (tRel 0))
+      (tXXi ℓf m⟨upRen_term_term ↑⟩⟨upRen_term_term ↑⟩[(tBox ℓ (tEval ℓf (tRel 0)))..] (tRel 0))
+      n (nat_to_term k)]
+| ellElimSubst {k ℓ P ht hf n b b'}: [L | b ⤳ b'] -> [L | tEllElim k ℓ P ht hf n b ⤳ tEllElim k ℓ P ht hf n b']
+| ellElimTrue {ℓ : ell} {k : newnat ℓ} {P ht hf n} :
+  [L | tEllElim k ℓ P ht hf n tTrue ⤳ ht[(tBox (cons_ell ℓ k true) (tEval ℓ n))..]]
+| ellElimFalse {ℓ : ell} {k : newnat ℓ} {P ht hf n} :
+  [L | tEllElim k ℓ P ht hf n tFalse ⤳ ht[(tBox (cons_ell ℓ k false) (tEval ℓ n))..]]
 
 where "[ L | t ⤳ t' ]" := (@OneRedAlg L t t') : typing_scope.
 
-Fixpoint OneRedAlg_rect_with_all
-  (L : list ell) (P : forall t t0 : term, [L | t ⤳ t0] -> Type)
-  (hBRed : forall A a t : term, P (tApp (tLambda A t) a) t[a..] BRed)
-  (happSubst : forall (t u a : term) (o : [L | t ⤳ u]), P t u o -> P (tApp t a) (tApp u a) (appSubst o))
-  (hnatElimSubst : forall (P0 hz hs n n' : term) (o : [L | n ⤳ n']),
-   P n n' o -> P (tNatElim P0 hz hs n) (tNatElim P0 hz hs n') (natElimSubst o))
-  (hnatElimZero : forall P0 hz hs : term, P (tNatElim P0 hz hs tZero) hz natElimZero)
-  (hnatElimSucc : forall P0 hz hs n : term,
-   P (tNatElim P0 hz hs (tSucc n)) (tApp (tApp hs n) (tNatElim P0 hz hs n)) natElimSucc)
-  (hboolElimSubst : forall (P0 ht hf n n' : term) (o : [L | n ⤳ n']),
-   P n n' o -> P (tBoolElim P0 ht hf n) (tBoolElim P0 ht hf n') (boolElimSubst o))
-  (hboolElimTrue : forall P0 ht hf : term, P (tBoolElim P0 ht hf tTrue) ht boolElimTrue)
-  (hboolElimFalse : forall P0 ht hf : term, P (tBoolElim P0 ht hf tFalse) hf boolElimFalse)
-  (halphaSubst : forall (i k : nat) (n n' : term) (o : [L | n ⤳ n']),
-   P n n' o -> P (tApp (tAlpha i) (nSucc k n)) (tApp (tAlpha i) (nSucc k n')) (alphaSubst o))
-  (halphaRed : forall (i : list_index L) (n : nat) (b : bool) (hin : in_ell (list_at L i) n b),
-   P (tApp (tAlpha i) (nat_to_term n)) (bool_to_term b) (alphaRed hin))
-  (hemptyElimSubst : forall (P0 e e' : term) (o : [L | e ⤳ e']),
-   P e e' o -> P (tEmptyElim P0 e) (tEmptyElim P0 e') (emptyElimSubst o))
-  (htreeElimSubst : forall (P0 hl hn t t' : term) (o : [L | t ⤳ t']),
-   P t t' o -> P (tTreeElim P0 hl hn t) (tTreeElim P0 hl hn t') (treeElimSubst o))
-  (htreeElimLeaf : forall P0 hl hn n : term, P (tTreeElim P0 hl hn (tLeaf n)) (tApp hl n) treeElimLeaf)
-  (htreeElimNode : forall P0 hl hn n tl tr : term,
-   P (tTreeElim P0 hl hn (tNode n tl tr))
-     (tApp (tApp (tApp (tApp (tApp hn n) tl) tr) (tTreeElim P0 hl hn tl)) (tTreeElim P0 hl hn tr))
-     treeElimNode)
-  (hfstSubst : forall (p p' : term) (o : [L | p ⤳ p']), P p p' o -> P (tFst p) (tFst p') (fstSubst o))
-  (hfstPair : forall A B a b : term, P (tFst (tPair A B a b)) a fstPair)
-  (hsndSubst : forall (p p' : term) (o : [L | p ⤳ p']), P p p' o -> P (tSnd p) (tSnd p') (sndSubst o))
-  (hsndPair : forall A B a b : term, P (tSnd (tPair A B a b)) b sndPair)
-  (hidElimRefl : forall A x P0 hr y A' z : term, P (tIdElim A x P0 hr y (tRefl A' z)) hr idElimRefl)
-  (hidElimSubst : forall (A x P0 hr y e e' : term) (o : [L | e ⤳ e']),
-   P e e' o -> P (tIdElim A x P0 hr y e) (tIdElim A x P0 hr y e') (idElimSubst o))
-  (hevalRel : forall (v k : nat) (b : bool) (ℓ : ell) (i : in_ell ℓ k b),
-   P (tApp (tEval ℓ (tRel v)) (nat_to_term k)) (bool_to_term b) (evalRel v k b ℓ i))
-  (hevalBox : forall (ℓ ℓ' : ell) (t : term), P (tEval ℓ (tBox ℓ' t)) t (evalBox ℓ ℓ' t))
-  (hxiSubst : forall (ℓ : ell) (n n' : term) k (o : [L | n ⤳ n']),
-   P n n' o -> P (tXi ℓ (nSucc k n)) (tXi ℓ (nSucc k n')) (xiSubst ℓ n n' k o))
-  (hxiLeaf : forall (ℓ : ell) (n : nat), P (tXi ℓ (nat_to_term n)) (tLeaf (nat_to_term n)) (xiLeaf ℓ n))
-  (hxiNode : forall (ℓ : ell) (n : term) (k : newnat ℓ) (w : whns k 0 n), whns_all (fun t t' => closure_all P) w ->
-   P (tXi ℓ n) (tNode (nat_to_term k) (tXi (cons_ell ℓ k true) n) (tXi (cons_ell ℓ k false) n))
-     (xiNode ℓ n k w))
-  (hxxiSubst : forall (ℓ : ell) (m m' n : term) (k : nat) (o : [L | m ⤳ m']), P m m' o ->
-   P (tXXi ℓ (nSucc k m) n) (tXXi ℓ (nSucc k m') n) (xxiSubst ℓ m m' n k o))
-  (t t0 : term) (o : [L | t ⤳ t0]) {struct o}: P t t0 o.
-Proof.
-  destruct o.
-  + eapply hBRed.
-  + eapply happSubst, OneRedAlg_rect_with_all; tea.
-  + eapply hnatElimSubst, OneRedAlg_rect_with_all; tea.
-  + eapply hnatElimZero.
-  + eapply hnatElimSucc.
-  + eapply hboolElimSubst, OneRedAlg_rect_with_all; tea.
-  + eapply hboolElimTrue.
-  + eapply hboolElimFalse.
-  + eapply halphaSubst, OneRedAlg_rect_with_all; tea.
-  + eapply halphaRed.
-  + eapply hemptyElimSubst, OneRedAlg_rect_with_all; tea.
-  + eapply htreeElimSubst, OneRedAlg_rect_with_all; tea.
-  + eapply htreeElimLeaf.
-  + eapply htreeElimNode.
-  + eapply hfstSubst, OneRedAlg_rect_with_all; tea.
-  + eapply hfstPair.
-  + eapply hsndSubst, OneRedAlg_rect_with_all; tea.
-  + eapply hsndPair.
-  + eapply hidElimRefl.
-  + eapply hidElimSubst, OneRedAlg_rect_with_all; tea.
-  + eapply hevalRel.
-  + eapply hevalBox.
-  + eapply hxiSubst, OneRedAlg_rect_with_all; tea.
-  + eapply hxiLeaf.
-  + eapply hxiNode, whns_all_forall, closure_all_forall, OneRedAlg_rect_with_all; tea.
-  + eapply hxxiSubst, OneRedAlg_rect_with_all; tea.
-Qed.
 
 
 (* Keep in sync with OneRedTermDecl! *)
 
 (** *** Multi-step reduction *)
 
-Definition RedClosureAlg {L : list ell} : term -> term -> Type := closure (@OneRedAlg L).
-(*   | redIdAlg {t} :
+Inductive RedClosureAlg {L : list ell} : term -> term -> Type :=
+  | redIdAlg {t} :
     [ L | t ⤳* t ]
   | redSuccAlg {t t' u} :
     [ L | t ⤳ t'] ->
     [ L | t' ⤳* u ] ->
     [ L | t ⤳* u ]
-  where *)
-Notation "[ L | t ⤳* t' ]" := (@RedClosureAlg L t t') : typing_scope.
+  where
+ "[ L | t ⤳* t' ]" := (@RedClosureAlg L t t') : typing_scope.
 
 Equations Derive Signature for OneRedAlg.
-Equations Derive Signature for closure.
+Equations Derive Signature for RedClosureAlg.
 
 
 #[export] Instance RedAlgTrans {L} : PreOrder (RedClosureAlg (L:=L)).
@@ -240,60 +126,8 @@ Record cored L t t' : Prop := { _ : [L |t' ⤳ t] }.
 (** *** Weak-head normal forms do not reduce *)
 
 Ltac inv_whne :=
-  match goal with [ H : whne _ |- _ ] => inversion H end.
+  match goal with [ H : whne _ _ |- _ ] => inversion H; block H end.
 
-
-Lemma whne_nored {L} n u :
-  @whne (@RedClosureAlg L) n -> [ L | n ⤳ u] -> False.
-Proof.
-  intros ne red.
-  induction ne in u, red |-*.
-  1-13: inversion red; subst; clear red.
-  all: try now inversion ne.
-  * inversion X.
-  * eapply nSucc_eq_inv in H1 as [[<- <-]| [(n0&->&<-)|(n0&<-&->)]].
-    - easy.
-    - inversion X.
-    - inversion ne.
-  * eapply nSucc_nat_to_term in H1 as [[] <-];
-    inversion ne.
-  * eapply nSucc_eq_inv in H1 as [[<- <-]| [(?&->&<-)|(?&<-&->)]].
-    - easy.
-    - inversion X.
-    - inversion ne.
-  * eapply nSucc_nat_to_term in H1 as [[] <-];
-    inversion ne.
-  * destruct k.
-    - admit.
-    - inversion X.
-Admitted.
-
-Ltac inv_alpha :=
-  match goal with
-    [ H : [_ | tAlpha _ ⤳ _] |- _ ] => inversion H
-    | [ H : whne (tAlpha _) |- _ ] => inversion H end.
-(* Lemma whnf_nored L n u :
-  @whnf (@RedClosureAlg L) n -> [ L | n ⤳ u] -> False.
-Proof.
-  intros nf red.
-  induction nf.
-  all: try now inversion red.
-  now eapply whne_nored.
-  admit.
-Admitted.
- *)
-(** *** Determinism of reduction *)
-
-Lemma ored_detaux : forall {L i i' n n'}, [ L | tApp (tAlpha i) (nat_to_term n) ⤳ tApp (tAlpha i') n'] -> False.
-Proof.
-  intros L i i' n n' H.
-  inversion H; subst; clear H.
-  * inversion X.
-  * eapply eq_sym, nSucc_nat_to_term in H2 as [[] <-].
-    - inversion X.
-    - inversion X.
-  * destruct b; inversion H3.
-Qed.
 
 #[local] Ltac nSucc_handler :=
 try match goal with
@@ -307,178 +141,81 @@ try match goal with
     eapply nat_to_term_inj in eq as <-
 end.
 
-(* Lemma det_closure L t n k v (r : [ L | t ⤳* n ]) : @whns (@RedClosureAlg L) k v n ->
-  closure_all (fun t u _ => (forall v, [L | t ⤳ v] -> u = v) /\
-    (forall k v : nat, @whns (@RedClosureAlg L) k v t -> False)) r ->
-    forall n' k' v', @whns (@RedClosureAlg L) k' v' n' ->[L | t ⤳* n' ] -> n = n'.
+Lemma whne_nored {L} n u nevar:
+  whne nevar n -> [ L | n ⤳ u] -> False.
 Proof.
-  intros w allr ??? w' r'.
-  induction r; inversion r'; subst; clear r'.
-  + reflexivity.
-  + cbn in allr. *)
-Goal forall L t, (forall u, [L | t ⤳ u] -> forall k v, @whns (@RedClosureAlg L) k v t -> False) ->
-  (forall u, [L | t ⤳* u] -> forall k v, @whns (@RedClosureAlg L) k v t -> t = u).
-Proof.
-  intros.
-  induction X.
-  reflexivity.
-  exfalso; eauto.
-Qed.
-
-(* Lemma wk_det L t n (r : [L | t ⤳* n]) :
-  (forall u, [L | t ⤳* u] ->forall k v, @whns (@RedClosureAlg L) k v t -> t = u) ->
-  closure_all (fun t u _ => (forall v, [L | t ⤳ v] -> u = v) /\
-    (forall k v : nat, @whns (@RedClosureAlg L) k v t -> False)) r ->
-  closure_all (fun t _ _ =>
-    forall u, [L | t ⤳* u] ->forall k v, @whns (@RedClosureAlg L) k v t -> t = u) r.
-Proof.
-  intros.
-  induction r.
-  + cbn in *. constructor.
-  + constructor.
-    - eapply IHr; clear IHr.
-      * cbn in X.
-        destruct r.
-       ++ cbn in *.
-          intros. *)
-
-Definition instant_det {L} t u (r : [L | t ⤳ u]) := (forall u', [L | t ⤳ u'] -> u = u')
-  /\ (forall k v, @whns (closure (@OneRedAlg L)) k v t -> False).
-
-
-
-Lemma whs_det L t n (r : [L | t ⤳* n]) :
-  (forall u (r : [L | n ⤳ u]), instant_det n u r) ->
-  closure_all (instant_det (L:=L)) r ->
-  forall k v, @whns (@RedClosureAlg L) k v n ->
-  forall n', [L | t ⤳* n'] ->
-  forall k' v', @whns (@RedClosureAlg L) k' v' n' ->
-  n = n'.
-Proof.
-  intros tdet allr ?? w ? r' ?? w'.
-  induction r; inversion r'; subst; clear r'.
-  + reflexivity.
-  + exfalso.
-    specialize (tdet _ X0) as []. eauto.
-  + destruct allr as (allr&hred&hwhns).
-    exfalso. eauto.
-  + destruct allr as (allr&hred&hwhns).
-    eapply IHr; tea.
-    now destruct (hred _ X0).
-Qed.
-
-
-Lemma whns_uniq_k L k v t (w : @whns (closure (@OneRedAlg L)) k v t) :
-  whns_all (fun _ _ => closure_all (instant_det (L:=L))) w ->
-  forall k', @whns (closure (@OneRedAlg L)) k' v t -> k = k'.
-Proof.
-(*   intros allw ? w'.
-  induction w' in k, w, allw |-*; revert allw; dependent inversion w; subst; cbn; clear w; intros ?; nSucc_handler; eauto.
-  all : try solve [inversion w'| inversion w0].
-  + admit.
-  + admit.
-  + inversion w'1.
-  + destruct (IHw'1 _ w0 ltac:(eapply allw)).
-    
-    eapply IHw'2.
-   destruct allw; eapply IHw'; tea. specialize (IHw' _ _ _ allw) as [<- ev].
-    now inversion ev.
-  + specialize (IHw' _ _ _ allw) as [<- ev].
-    now inversion ev.
-  + destruct allw as (allw1&hr&allw2).
-    specialize (IHw' _ _ _ allw1) as [<- ev].
-    now inversion ev.
-  + specialize (IHw'1 _ _ _ allw) as [<- ev].
-    now inversion ev.
-  + inversion w'1.
-  + destruct allw as (allw0&allc&allw1).
-    assert (forall t' (r : [L | n' ⤳ t']), instant_det n' t' r).
-    { intros.
-      split.
-      - intros. *)
-Admitted.
-
-
-Lemma whns_uniq_kv L k v t (w : @whns (closure (@OneRedAlg L)) k v t) :
-  whns_all (fun _ _ => closure_all (instant_det (L:=L))) w ->
-  forall k' v', @whns (closure (@OneRedAlg L)) k' v' t -> k = k' /\ v = v'.
-Proof.
-  intros allw ?? w'.
-  induction w' in k, v, w, allw |-*; revert allw; dependent inversion w; subst; cbn; clear w; intros ?; nSucc_handler; eauto.
-  all : try solve [inversion w'| inversion w0].
-  + specialize (IHw' _ _ _ allw) as [<- ev].
-    now inversion ev.
-  + specialize (IHw' _ _ _ allw) as [<- ev].
-    now inversion ev.
-  + destruct allw as (allw1&hr&allw2).
-    specialize (IHw' _ _ _ allw1) as [<- ev].
-    now inversion ev.
-  + specialize (IHw'1 _ _ _ allw) as [<- ev].
-    now inversion ev.
-  + inversion w'1.
-  + destruct allw as (allw0&allc&allw1).
-    assert (forall t' (r : [L | n' ⤳ t']), instant_det n' t' r).
-    { intros.
-      split.
-      - intros.
-
-Admitted.
-
-Lemma ored_no_whns {L t u} :
-  [L | t ⤳ u] -> forall k v, @whns (@RedClosureAlg L) k v t -> False.
-Proof.
-  intros red k v w.
-  induction red using OneRedAlg_rect_with_all in k, v, w |-*;
-    inversion w; subst; clear w; nSucc_handler; eauto.
-  all: try solve [inversion X |inversion red].
+  intros ne red.
+  induction ne in u, red |-*.
+  1-14: inversion red; subst; clear red; nSucc_handler.
+  all: try solve [now inversion ne | now inversion H2].
   * destruct (notin_is_not_in ltac:(tea) ltac:(tea)).
-  * destruct k'.
-    2: inversion w0.
-    cbn in w0.
-    admit.
-Admitted.
-
-Lemma ored_det {L t u} :
-  [L | t ⤳ u] -> (forall v, [L | t ⤳ v] ->
-  u = v) /\ (forall k v, @whns (@RedClosureAlg L) k v t -> False).
-Proof.
-  intros red.
-  induction red using OneRedAlg_rect_with_all; try destruct IHred as [IHredred IHredwhns].
-  1-26 : split;
-    [intros t_r red'; inversion red'; subst; clear red'; nSucc_handler; repeat f_equal; eauto
-    |intros k_w v_w wt; inversion wt; subst; clear wt; nSucc_handler; eauto]; try solve [inversion X | inversion red].
-  * eapply index_to_nat_inj in H0 as <-.
-    eapply functionality; tea.
-  * eapply functionality; tea.
-  * destruct (notin_is_not_in H0 i).
   * destruct k.
-    2: inversion X.
-    destruct (IHredwhns _ _ X).
-  * destruct n; inversion X.
-  * destruct k0.
-    2: inversion w.
-    exfalso; cbn in *.
-    induction w in X, n', X0 |-* ; inversion X0; subst; clear X0; nSucc_handler.
-    all: try solve [inversion X1 | inversion w | eapply IHw; tea].
-    + destruct (notin_is_not_in n H3).
-    + destruct k'.
-      2: inversion X1.
-      cbn in *.
-      specialize (IHw X).
-      admit.
-    + destruct X as (?&?&?).
-      eapply IHw1; tea.
-    + inversion w1.
-  * destruct n0; inversion w.
-  * admit.
-  * admit.
-  * admit.
-  * destruct k'.
-    2: inversion w.
-    cbn in w.
-Admitted.
+    2: inversion H2.
+    pose proof (nevar_uniq ne H2).
+    destruct nevar; inversion H.
+  * inversion H3.
+  * destruct k.
+    2: inversion H3.
+    pose proof (nevar_uniq ne H3).
+    destruct nevar; inversion H.
+Qed.
 
-Lemma red_whne {L} t u : [ L | t ⤳* u] -> whne t -> t = u.
+Ltac inv_alpha :=
+  match goal with
+    [ H : [_ | tAlpha _ ⤳ _] |- _ ] => inversion H
+    | [ H : whne (tAlpha _) |- _ ] => inversion H end.
+Lemma whnf_nored L n u :
+  @whnf n -> [ L | n ⤳ u] -> False.
+Proof.
+  intros nf red.
+  induction nf.
+  all: try now inversion red.
+  now eapply whne_nored.
+Qed.
+
+(** *** Determinism of reduction *)
+
+(* Lemma ored_detaux : forall {L i i' n n'}, [ L | tApp (tAlpha i) (nat_to_term n) ⤳ tApp (tAlpha i') n'] -> False.
+Proof.
+  intros L i i' n n' H.
+  inversion H; subst; clear H.
+  * inversion X.
+  * eapply eq_sym, nSucc_nat_to_term in H2 as [[] <-].
+    - inversion X.
+    - inversion X.
+  * destruct b; inversion H3.
+Qed. *)
+
+
+Lemma ored_det {L t u v} :
+  [L | t ⤳ u] -> [L | t ⤳ v] -> u = v.
+Proof.
+  intros red red'.
+  induction red in v, red' |-*.
+  all: depelim red'; nSucc_handler; eauto.
+(*   1-29: inversion red'; subst; clear red'; nSucc_handler; eauto. *)
+(*   71-72 : depelim red'. *)
+  all : try solve [repeat f_equal; eauto].
+  all : repeat match goal with r : [_ | _ ⤳ _] |- _ => try solve [inversion r]; block r | _ => idtac end; unblock.
+  all : try match goal with w : whne _ (nSucc ?k _) |- _ => destruct k; [ | inversion w]; cbn in w end .
+  all : try match goal with w : whne _ (nat_to_term ?k) |- _ => destruct k; inversion w end .
+  all: try solve [exfalso; eapply whne_nored; eauto].
+  * eapply index_to_nat_inj in H as <-.
+    eapply f_equal, functionality; tea.
+  * eapply f_equal, functionality; tea.
+  * pose proof (nevar_uniq w w0).
+    destruct k as [k wf], k0 as [k0 wf0]; cbn in *.
+    now inversion H; subst.
+  * pose proof (nevar_uniq w w0).
+    destruct k as [k wf], k0 as [k0 wf0]; cbn in *.
+    now inversion H; subst.
+  * destruct k as [k wf], k0 as [k0 wf0]; cbn in *.
+    now inversion H; subst.
+  * destruct k as [k wf], k0 as [k0 wf0]; cbn in *.
+    now inversion H; subst.
+Qed.
+
+Lemma red_whne {L} t u nevar : [ L | t ⤳* u] -> whne nevar t -> t = u.
 Proof.
   intros [] ?.
   1: reflexivity.
@@ -528,14 +265,7 @@ Proof.
   all: try now constructor.
   rewrite <- ren_index_to_ren with (wρε := wρε).
   constructor.
-  eapply well_Fwk_in. , hin.
-  2-10, 12-21: now constructor.
-  - rewrite subst_ren_alpha. constructor.
-  - cbn.
-    rewrite nat_to_term_ren_alpha, bool_to_term_ren_alpha,
-      <- ren_index_to_ren with (wρε:=wρε).
-    eapply alphaRed.
-    eapply well_Fwk_in, hin.
+  eapply well_Fwk_in; tea.
 Defined.
 
 Lemma oredalg_wk (ρ : nat -> nat) L (t u : term) :
@@ -544,12 +274,20 @@ Lemma oredalg_wk (ρ : nat -> nat) L (t u : term) :
 Proof.
   intros Hred.
   induction Hred in ρ |- *.
-  2-9,12-21:cbn; now econstructor.
-  - cbn. rewrite subst_ren_up.
-    constructor.
-  - cbn. eapply alphaSubstSucc, IHHred.
-  - cbn. rewrite nat_to_term_ren, bool_to_term_ren.
-    now econstructor.
+  all: cbn.
+  all: rewrite ? nSucc_ren, ? subst_ren_up,
+    ? nat_to_term_ren, ? bool_to_term_ren.
+  all: try now econstructor.
+  - econstructor.
+    exact (whne_ren _ _ _ w).
+  - cbn. simpl. repeat (unfold funcomp; cbn).
+    replace m⟨upRen_term_term ↑⟩⟨upRen_term_term (upRen_term_term ρ)⟩
+      with m⟨upRen_term_term ρ⟩⟨upRen_term_term ↑⟩.
+    replace m⟨upRen_term_term ↑⟩⟨upRen_term_term ↑⟩⟨upRen_term_term (upRen_term_term (upRen_term_term ρ))⟩
+      with m⟨upRen_term_term ρ⟩⟨upRen_term_term ↑⟩⟨upRen_term_term ↑⟩.
+    refine (xxiNode _).
+    { exact (whne_ren _ _ _ w). }
+    all: now bsimpl.
 Qed.
 (* 
 Lemma oredalg_str (Γ Δ : context) (ρ : Δ ≤ Γ) (t u : term) :
@@ -568,8 +306,8 @@ Proof.
   all: eexists ; split ; cycle -1 ; [now econstructor | now bsimpl].
 Qed. *)
 
-Lemma cFredalg L L' ρε (wρε : well_Fweakening ρε L' L) t u: 
-  [L | t ⤳* u] -> [L' | ren_alpha ρε t ⤳* ren_alpha ρε u].
+Lemma cFredalg L L' (wρε : well_Fweakening L' L) t u: 
+  [L | t ⤳* u] -> [L' | t ⤳* u].
 Proof.
   induction 1; econstructor; eauto using oFredalg.
 Defined.
@@ -664,7 +402,7 @@ Proof.
   econstructor; tea; now constructor.
 Qed.
 
-Lemma redalg_alpha {L i t t'} : [L | t ⤳* t'] -> [L | tApp (tAlpha i) t ⤳* tApp (tAlpha i) t'].
+(* Lemma redalg_alpha {L i t t'} : [L | t ⤳* t'] -> [L | tApp (tAlpha i) t ⤳* tApp (tAlpha i) t'].
 Proof.
   induction 1; [reflexivity|].
   econstructor; tea; now econstructor.
@@ -693,7 +431,7 @@ Proof.
   - tea.
   - eauto using redalg_alphaSucc.
 Qed.
-
+ *)
 
 Lemma redalg_one_step {L t t'} : [ L | t ⤳ t'] -> [ L | t ⤳* t'].
 Proof. intros; econstructor;[tea|reflexivity]. Qed.
@@ -717,8 +455,7 @@ Proof.
   inversion red ; subst ; clear red.
   - exfalso.
     inversion nf ; subst ; clear nf.
-    inversion H ; subst ; clear H.
-    inversion H1 ; subst ; clear H1.
+    repeat inv_whne.
   - inversion H ; subst.
     2: now inversion H4.
     refold.
@@ -737,8 +474,7 @@ Proof.
   inversion red ; subst ; clear red.
   - exfalso.
     inversion nf ; subst ; clear nf.
-    inversion H ; subst ; clear H.
-    inversion H1 ; subst ; clear H1.
+    repeat inv_whne.
   - inversion H ; subst.
     1: now inversion H2.
     eassumption.
@@ -754,8 +490,7 @@ Proof.
   inversion red ; subst ; clear red.
   - exfalso.
     inversion nf ; subst ; clear nf.
-    inversion H ; subst ; clear H.
-    inversion H1 ; subst ; clear H1.
+    repeat inv_whne.
   - inversion H ; subst.
     1: now inversion H2.
     eassumption.
